translator/lean/llzk/Llzk/Language/Core/Analysis/Liveness.lean
@@ -1,0 +1,194 @@
+import Llzk.Basic
+import Llzk.Language.Core.Syntax.AST
+import Std.Data.TreeSet.Basic
+
+/- This module implements liveness analysis for the core language. The liveness information
+   is stored in the metadata of each command and function.
+
+   The main function is `addLivenessProg` which takes a program and returns a new program
+   with liveness information added to each function. The liveness information of each function
+   is computed by traversing the commands in reverse order and keeping track of the live
+   variables at each point.
+
+   Traversing in reverse order is done for now with recursion, we should consider
+   reversing the list and use tail-recursion.
+-/
+
+namespace Llzk.Language.Core.Analysis.Liveness
+
+open Llzk.Language.Core.Syntax.AST
+
+
+def addUsedVarsSimpleExpr {c : ZKConfig} (vars : VarIDSet) (s : SimpleExpr c) : VarIDSet :=
+    match s with
+    | SimpleExpr.var id => vars.insert id
+    | _ => vars
+
+def addUsedVarsSimpleExprs {c : ZKConfig} (vars : VarIDSet) (ss : List (SimpleExpr c)) : VarIDSet :=
+    match ss with
+    | [] => vars
+    | s :: rest => addUsedVarsSimpleExprs (addUsedVarsSimpleExpr vars s) rest
+
+def addUsedVarsExpr {c : ZKConfig} (vars : VarIDSet) (e : Expr c) : VarIDSet :=
+    match e with
+    | .id s => addUsedVarsSimpleExpr vars s
+    | .neg s => addUsedVarsSimpleExpr vars s
+    | .add s1 s2 => addUsedVarsSimpleExpr (addUsedVarsSimpleExpr vars s1) s2
+    | .sub s1 s2 => addUsedVarsSimpleExpr (addUsedVarsSimpleExpr vars s1) s2
+    | .mul s1 s2 => addUsedVarsSimpleExpr (addUsedVarsSimpleExpr vars s1) s2
+    | .div s1 s2 => addUsedVarsSimpleExpr (addUsedVarsSimpleExpr vars s1) s2
+    | .shl s1 s2 => addUsedVarsSimpleExpr (addUsedVarsSimpleExpr vars s1) s2
+    | .shr s1 s2 => addUsedVarsSimpleExpr (addUsedVarsSimpleExpr vars s1) s2
+    | .and s1 s2 => addUsedVarsSimpleExpr (addUsedVarsSimpleExpr vars s1) s2
+    | .or s1 s2 => addUsedVarsSimpleExpr (addUsedVarsSimpleExpr vars s1) s2
+    | .xor s1 s2 => addUsedVarsSimpleExpr (addUsedVarsSimpleExpr vars s1) s2
+    | .not s => addUsedVarsSimpleExpr vars s
+    | .True => vars
+    | .False => vars
+    | .eq s1 s2 => addUsedVarsSimpleExpr (addUsedVarsSimpleExpr vars s1) s2
+    | .neq s1 s2 => addUsedVarsSimpleExpr (addUsedVarsSimpleExpr vars s1) s2
+    | .lt s1 s2 => addUsedVarsSimpleExpr (addUsedVarsSimpleExpr vars s1) s2
+    | .gt s1 s2 => addUsedVarsSimpleExpr (addUsedVarsSimpleExpr vars s1) s2
+    | .le s1 s2 => addUsedVarsSimpleExpr (addUsedVarsSimpleExpr vars s1) s2
+    | .ge s1 s2 => addUsedVarsSimpleExpr (addUsedVarsSimpleExpr vars s1) s2
+    | .bor s1 s2 => addUsedVarsSimpleExpr (addUsedVarsSimpleExpr vars s1) s2
+    | .band s1 s2 => addUsedVarsSimpleExpr (addUsedVarsSimpleExpr vars s1) s2
+    | .bneg s => addUsedVarsSimpleExpr vars s
+
+def addUsedVarsCond {c : ZKConfig} (vars : VarIDSet) (cond : Cond c) : VarIDSet :=
+    match cond with
+    | .eq s1 s2 => addUsedVarsSimpleExpr (addUsedVarsSimpleExpr vars s1) s2
+    | .neq s1 s2 => addUsedVarsSimpleExpr (addUsedVarsSimpleExpr vars s1) s2
+
+
+def getCmdsLiveIn {c : ZKConfig} (cmds : List (ComWithMD c)) : VarIDSet :=
+    match cmds with
+    | [] => emptyVarIDSet
+    | i :: _ =>
+        match i with
+        | .mk md _ => md.liveness.live_in
+
+def eraseVars (vars : VarIDSet) (varsToErase : List VarID) : VarIDSet :=
+    match varsToErase with
+    | [] => vars
+    | v :: rest => eraseVars (vars.erase v) rest
+
+def addParams (vars : VarIDSet) (params : List Param) : VarIDSet :=
+    match params with
+    | [] => vars
+    | p :: rest => addParams (vars.insert p.name) rest
+
+def eraseParams (vars : VarIDSet) (params : List Param) : VarIDSet :=
+    match params with
+    | [] => vars
+    | p :: rest => eraseParams (vars.erase p.name) rest
+
+mutual
+
+def addLivenessCmd {c : ZKConfig} (i : ComWithMD c) (out : VarIDSet) :=
+    match i with
+    | .mk md cmd =>
+        match cmd with
+        | .skip =>
+          ComWithMD.mk { md with liveness := { live_in := out, live_out := out } } cmd
+        | .assign id e =>
+          let out' := out.erase id
+          let liveIn := addUsedVarsExpr out' e
+          dbg_trace s!"Assign: {id} := {e}, live_out: {out}, live_in: {liveIn} {out'}"
+          ComWithMD.mk { md with liveness := { live_in := liveIn, live_out := out } } cmd
+        | .if_stmt cond tb eb =>
+          let tb' := addLivenessCmds tb out
+          let eb' := addLivenessCmds eb out
+          let liveInThen := getCmdsLiveIn tb'
+          let liveInElse := getCmdsLiveIn eb'
+          let liveIn := addUsedVarsCond (liveInThen.union liveInElse) cond
+          let cmd' := Com.if_stmt cond tb' eb'
+          ComWithMD.mk { md with liveness := { live_in := liveIn, live_out := out } } cmd'
+        | .with_const _id _e body =>
+          -- Variable 'id' is not considered since it is a constant variable. Also 'e'
+          -- is not considered since it is supposed to be a constant expression.
+          let body' := addLivenessCmds body out
+          let liveIn := getCmdsLiveIn body'
+          let cmd' := Com.with_const _id _e body'
+          ComWithMD.mk { md with liveness := { live_in := liveIn, live_out := out } } cmd'
+        | .loop_exp _idx _start _rep _step body =>
+          -- None of the expressions are considered since they are supposed to be constant
+          -- expressions. Also the loop variable 'idx' is not considered since it is a
+          -- constant variable. We need to iterate the loop twice to get the fixed point of the
+          -- live variables.
+          let body' := addLivenessCmds body out
+          let liveIn := getCmdsLiveIn body'
+          let body'' := addLivenessCmds body (liveIn.union out)
+          let liveIn' := getCmdsLiveIn body''
+          let cmd' := Com.loop_exp _idx _start _rep _step body''
+          ComWithMD.mk { md with liveness := { live_in := liveIn', live_out := out } } cmd'
+        | .loop _idx _start _rep _step body =>
+          -- The loop variable 'idx' is not considered since it is a constant variable.
+          -- We need to iterate the loop twice to get the fixed point of the live variables.
+          let body' := addLivenessCmds body out
+          let liveIn := getCmdsLiveIn body'
+          let body'' := addLivenessCmds body (liveIn.union out)
+          let liveIn' := getCmdsLiveIn body''
+          let cmd' := Com.loop _idx _start _rep _step body''
+          ComWithMD.mk { md with liveness := { live_in := liveIn', live_out := out } } cmd'
+        | .new_array id _size =>
+        -- We do not consider size since it is supposed to be a constant expression.
+          let liveIn := out.erase id
+          ComWithMD.mk { md with liveness := { live_in := liveIn, live_out := out } } cmd
+        | .read_array id arr idx => -- id := arr[idx]
+          let out' := out.erase id
+          let liveIn := out'.insert arr
+          let liveIn' := addUsedVarsSimpleExpr liveIn idx
+          ComWithMD.mk { md with liveness := { live_in := liveIn', live_out := out } } cmd
+        | .write_array arr idx val => -- arr[idx] := val
+            -- Note that 'arr' is considered live-in since it is an array access
+            let liveIn := out.insert arr
+            let liveIn' := addUsedVarsSimpleExpr liveIn idx
+            let liveIn'' := addUsedVarsSimpleExpr liveIn' val
+            ComWithMD.mk { md with liveness := { live_in := liveIn'', live_out := out } } cmd
+        | .copy_array dst src =>
+          let liveIn := out.erase dst
+          let liveIn' := liveIn.insert src
+          ComWithMD.mk { md with liveness := { live_in := liveIn', live_out := out } } cmd
+        | .func_call rets _id args =>
+          let out' := eraseVars out rets
+          let liveIn := addUsedVarsSimpleExprs out' args
+          ComWithMD.mk { md with liveness := { live_in := liveIn, live_out := out } } cmd
+
+
+def addLivenessCmds {c : ZKConfig} (cmds : List (ComWithMD c)) (out : VarIDSet) :=
+    match cmds with
+    | [] => []
+    | [i] => [addLivenessCmd i out]
+    | i :: rest =>
+        let rest' := addLivenessCmds rest out
+        let out' := getCmdsLiveIn rest'
+        let i' := addLivenessCmd i out'
+        i' :: rest'
+end
+
+
+
+def addLivenessFunc {c : ZKConfig} (f : FuncWithMD c) : FuncWithMD c :=
+    match f with
+    | .mk md func =>
+    match func with
+     | Func.mk name params rets body =>
+     let out := addParams emptyVarIDSet rets
+     let body' := addLivenessCmds body out
+     let liveIn := getCmdsLiveIn body'
+     let func' := Func.mk name params rets body'
+     FuncWithMD.mk { md with liveness := { live_in := liveIn, live_out := out } } func'
+
+def addLivenessFuncs {c : ZKConfig} (funcs : List (FuncWithMD c)) : List (FuncWithMD c) :=
+    match funcs with
+    | [] => []
+    | f :: rest => addLivenessFunc f :: addLivenessFuncs rest
+
+def addLivenessProg {c : ZKConfig} (p : ProgWithMD c) : ProgWithMD c :=
+    match p with
+    | .mk md funcs =>
+        let funcs' := addLivenessFuncs funcs
+        ProgWithMD.mk md funcs'
+
+end Llzk.Language.Core.Analysis.Liveness
